\documentclass[12pt]{article}
\pagestyle{empty}
\begin{document}
At $n=1$, the statement is obviously true.

At $n=2$, 
$
{\left[ \begin{array}{cc}
	0 & 1 \\
	1 & 1 \end{array} \right]}^2
=
\left[ \begin{array}{cc}
	1 & 1 \\
	1 & 2 \end{array} \right]
$
, which agrees with the formula.

Next, it is straightforward to prove the general case, when $n>2$:

\begin{eqnarray*}
{\left[ \begin{array}{cc}
	0 & 1 \\
	1 & 1 \end{array} \right]}^n
&=& 
\left[ \begin{array}{cc}
	f_{n-2}	&	f_{n-1} \\
	f_{n-1}	&	f_n \end{array} \right]
\left[ \begin{array}{cc}
	0 & 1 \\
	1 & 1 \end{array} \right]
\\
&=&
\left[ \begin{array}{cc}
	f_{n-1}	&	f_{n-1} + f_{n-2} \\
	f_n	&	f_{n+1} \end{array} \right]
\\
&=&
\left[ \begin{array}{cc}
	f_{n-1}	&	f_n \\
	f_n	&	f_{n+1} \end{array} \right]
\end{eqnarray*}

...which concludes the proof.
\end{document}
