\documentclass[12pt]{article}
\pagestyle{empty}
\begin{document}
At $n=1$ and $n=2$, $f_n$ is correct.

At $n=3$, $f_2^2 + f_1^2 = 1^2 + 1^2 = 2$, which is correct.

At $n=4$, $f_3^2 - f_1^2 = 4 - 1 = 3$, which is correct.

When n is odd:

\begin{eqnarray*}
f_n &=& f_{n-1} + f_{n-2} \\
    &=& \left( f_{\frac{n-1}{2}+1}^2 - f_{\frac{n-1}{2}-1}^2 \right)
        + \left( f_{\frac{n-1}{2}}^2 + f_{\frac{n-3}{2}}^2 \right)
	\mbox{ since $n-1$ is even and $n-2$ is odd} \\
    &=& f_{\frac{n+1}{2}}^2 - f_{\frac{n-3}{2}}^2
        + f_{\frac{n-1}{2}}^2 + f_{\frac{n-3}{2}}^2 \\
    &=& f_{\frac{n+1}{2}}^2 + f_{\frac{n-1}{2}}^2
\end{eqnarray*}

When n is even:

\begin{eqnarray*}
f_n &=& f_{n-1} + f_{n-2} \\
    &=& f_{\frac{n-1+1}{2}}^2 + f_{\frac{n-1-1}{2}}^2
        + f_{\frac{n-2}{2}+1}^2 - f_{\frac{n-2}{2}-1}^2
	\mbox{ since $n-1$ is odd and $n-2$ is even} \\
    &=& 2f_{\frac{n}{2}}^2 + f_{\frac{n}{2}-1}^2 - f_{\frac{n}{2}-2}^2 \\
    &=& 2f_{\frac{n}{2}}^2
        + {\left( f_{\frac{n}{2}} - f_{\frac{n}{2}-2} \right)}^2
	- f_{\frac{n-2}{2}-2}^2 \\
    &=& 2f_{\frac{n}{2}}^2 + f_{\frac{n}{2}}^2
        - 2f_{\frac{n}{2}}f_{\frac{n}{2}-2} + f_{\frac{n}{2}-2}^2
	- f_{\frac{n}{2}-2}^2 \\
    &=& 3f_{\frac{n}{2}}^2 - 2f_{\frac{n}{2}}f_{\frac{n}{2}-2} \\
    &=& f_{\frac{n}{2}}
        {\left( 3f_{\frac{n}{2}} - 2f_{\frac{n}{2}-2} \right)} \\
    &=& f_{\frac{n}{2}}{\left( f_{\frac{n}{2}} + 2f_{\frac{n}{2}-1} \right)} \\
    &=& f_{\frac{n}{2}}{\left( f_{\frac{n}{2}+1} + f_{\frac{n}{2}-1} \right)} \\
    &=& {\left( f_{\frac{n}{2}+1} - f_{\frac{n}{2}-1} \right)}
        {\left( f_{\frac{n}{2}+1} + f_{\frac{n}{2}-1} \right)} \\
    &=& f_{\frac{n}{2}-1}^2 - f_{\frac{n}{2}+1}^2
\end{eqnarray*}
\end{document}
